completely remake AsyncSectorDiskModel

BlockCacheSystem/AsyncSectorDiskModel.i.dfy
@@ -3,6 +3,7 @@ include "../lib/Base/Maps.s.dfy"
 include "../PivotBetree/Bounds.i.dfy"
 include "DiskLayout.i.dfy"
 include "SectorType.i.dfy"
+include "JournalDisk.i.dfy"
 
 //
 // An AsyncSectorDiskModel allows concurrent outstanding I/Os to a disk where each "sector"
@@ -26,6 +27,7 @@ module AsyncSectorDisk {
   import opened JournalRanges
   import opened PivotBetreeGraph
   import opened Sequences
+  import opened JournalDisk
 
   type ReqId = uint64
 
@@ -40,8 +42,6 @@ module AsyncSectorDisk {
 
   datatype ReqWriteSuperblockId = ReqWriteSuperblockId(id: ReqId, req: ReqWriteSuperblock)
 
-  datatype RespReadSuperblockId = RespReadSuperblockId(id: ReqId, superblock: Option<Superblock>)
-
   datatype DiskOp =
     | ReqReadSuperblockOp(id: ReqId, which: int)
     | ReqReadJournalOp(id: ReqId, reqReadJournal: ReqReadJournal)
@@ -50,9 +50,6 @@ module AsyncSectorDisk {
 
     | ReqWriteSuperblockOp(id: ReqId, which: int, reqWriteSuperblock: ReqWriteSuperblock)
     | ReqWriteJournalOp(id: ReqId, reqWriteJournal: ReqWriteJournal)
-    | ReqWriteJournalOp2(
-      id1: ReqId, reqWriteJournal1: ReqWriteJournal,
-      id2: ReqId, reqWriteJournal2: ReqWriteJournal)
     | ReqWriteIndirectionTableOp(id: ReqId, reqWriteIndirectionTable: ReqWriteIndirectionTable)
     | ReqWriteNodeOp(id: ReqId, reqWriteNode: ReqWriteNode)
 
@@ -76,23 +73,11 @@ module AsyncSectorDisk {
     reqReadIndirectionTables: map<ReqId, ReqReadIndirectionTable>,
     reqReadNodes: map<ReqId, ReqReadNode>,
 
-    reqWriteSuperblock1: Option<ReqWriteSuperblockId>,
-    reqWriteSuperblock2: Option<ReqWriteSuperblockId>,
-    reqWriteJournals: map<ReqId, ReqWriteJournal>,
-    reqWriteIndirectionTables: map<ReqId, ReqWriteIndirectionTable>,
-    reqWriteNodes: map<ReqId, ReqWriteNode>,
-
-    respReadSuperblock1: Option<RespReadSuperblockId>,
-    respReadSuperblock2: Option<RespReadSuperblockId>,
-    respReadJournals: map<ReqId, Option<JournalRange>>,
-    respReadIndirectionTables: map<ReqId, Option<IndirectionTable>>,
-    respReadNodes: map<ReqId, Option<Node>>,
-
-    respWriteSuperblock1: Option<ReqId>,
-    respWriteSuperblock2: Option<ReqId>,
-    respWriteJournals: set<ReqId>,
-    respWriteIndirectionTables: set<ReqId>,
-    respWriteNodes: set<ReqId>,
+    reqWriteSuperblock1: Option<ReqId>,
+    reqWriteSuperblock2: Option<ReqId>,
+    reqWriteJournals: map<ReqId, JournalIndices>,
+    reqWriteIndirectionTables: map<ReqId, Location>,
+    reqWriteNodes: map<ReqId, Location>,
 
     // The disk:
     superblock1: Option<Superblock>,
@@ -115,18 +100,6 @@ module AsyncSectorDisk {
     && s.reqWriteJournals == map[]
     && s.reqWriteIndirectionTables == map[]
     && s.reqWriteNodes == map[]
-
-    && s.respReadSuperblock1 == None
-    && s.respReadSuperblock2 == None
-    && s.respReadJournals == map[]
-    && s.respReadIndirectionTables == map[]
-    && s.respReadNodes == map[]
-
-    && s.respWriteSuperblock1 == None
-    && s.respWriteSuperblock2 == None
-    && s.respWriteJournals == {}
-    && s.respWriteIndirectionTables == {}
-    && s.respWriteNodes == {}
   }
 
   ///////// RecvRead
@@ -136,8 +109,6 @@ module AsyncSectorDisk {
     && dop.ReqReadSuperblockOp?
     && Some(dop.id) != s.reqReadSuperblock1
     && Some(dop.id) != s.reqReadSuperblock2
-    && (s.respReadSuperblock1.Some? ==> s.respReadSuperblock1.value.id != dop.id)
-    && (s.respReadSuperblock2.Some? ==> s.respReadSuperblock2.value.id != dop.id)
     && (dop.which == 0 || dop.which == 1)
     && (dop.which == 0 ==>
       s' == s.(reqReadSuperblock1 := Some(dop.id)))
@@ -149,7 +120,6 @@ module AsyncSectorDisk {
   {
     && dop.ReqReadJournalOp?
     && dop.id !in s.reqReadJournals
-    && dop.id !in s.respReadJournals
     && 0 <= dop.reqReadJournal.start < NumJournalBlocks() as int
     && 0 <= dop.reqReadJournal.start + dop.reqReadJournal.len <= NumJournalBlocks() as int
     && s' == s.(reqReadJournals := s.reqReadJournals[dop.id := dop.reqReadJournal])
@@ -159,7 +129,6 @@ module AsyncSectorDisk {
   {
     && dop.ReqReadIndirectionTableOp?
     && dop.id !in s.reqReadIndirectionTables
-    && dop.id !in s.respReadIndirectionTables
     && s' == s.(reqReadIndirectionTables := s.reqReadIndirectionTables[dop.id := dop.reqReadIndirectionTable])
   }
 
@@ -167,7 +136,6 @@ module AsyncSectorDisk {
   {
     && dop.ReqReadNodeOp?
     && dop.id !in s.reqReadNodes
-    && dop.id !in s.respReadNodes
     && s' == s.(reqReadNodes := s.reqReadNodes[dop.id := dop.reqReadNode])
   }
 
@@ -176,61 +144,59 @@ module AsyncSectorDisk {
   predicate RecvWriteSuperblock(k: Constants, s: Variables, s': Variables, dop: DiskOp)
   {
     && dop.ReqWriteSuperblockOp?
-    && Some(dop.id) != s.respWriteSuperblock1
-    && Some(dop.id) != s.respWriteSuperblock2
-    && (s.reqWriteSuperblock1.Some? ==> s.reqWriteSuperblock1.value.id != dop.id)
-    && (s.reqWriteSuperblock2.Some? ==> s.reqWriteSuperblock2.value.id != dop.id)
+    && (s.reqWriteSuperblock1.Some? ==> s.reqWriteSuperblock1.value != dop.id)
+    && (s.reqWriteSuperblock2.Some? ==> s.reqWriteSuperblock2.value != dop.id)
     && (dop.which == 0 || dop.which == 1)
     && (dop.which == 0 ==>
-      s' == s.(reqWriteSuperblock1 := Some(ReqWriteSuperblockId(dop.id, dop.reqWriteSuperblock))))
+      s' == s.(reqWriteSuperblock1 := Some(dop.id))
+             .(superblock1 := Some(dop.reqWriteSuperblock.superblock))
+    )
     && (dop.which == 1 ==>
-      s' == s.(reqWriteSuperblock2 := Some(ReqWriteSuperblockId(dop.id, dop.reqWriteSuperblock))))
+      s' == s.(reqWriteSuperblock2 := Some(dop.id))
+             .(superblock2 := Some(dop.reqWriteSuperblock.superblock))
+    )
   }
 
-  predicate ValidReqWriteJournal(reqWriteJournal: ReqWriteJournal)
+  predicate ValidJournalIndices(indices: JournalIndices)
   {
-    && 0 <= reqWriteJournal.start < NumJournalBlocks() as int
-    && 0 <= reqWriteJournal.start + |reqWriteJournal.journal| <= NumJournalBlocks() as int
+    && 0 <= indices.start < NumJournalBlocks() as int
+    && 0 <= indices.len <= NumJournalBlocks() as int
   }
 
   predicate RecvWriteJournal(k: Constants, s: Variables, s': Variables, dop: DiskOp)
   {
     && dop.ReqWriteJournalOp?
     && dop.id !in s.reqWriteJournals
-    && dop.id !in s.respWriteJournals
-    && ValidReqWriteJournal(dop.reqWriteJournal)
-    && s' == s.(reqWriteJournals := s.reqWriteJournals[dop.id := dop.reqWriteJournal])
+    && var indices := JournalIndices(dop.reqWriteJournal.start, |dop.reqWriteJournal.journal|);
+    && JournalUpdate(s.journal, s'.journal, indices, dop.reqWriteJournal.journal)
+    && s' == s.(reqWriteJournals := s.reqWriteJournals[dop.id := indices])
+              .(journal := s'.journal)
   }
 
-  predicate RecvWriteJournal2(k: Constants, s: Variables, s': Variables, dop: DiskOp)
+  predicate DiskMapUpdate<T>(disk: imap<Location, T>, disk': imap<Location, T>, updateLoc: Location, t: T)
   {
-    && dop.ReqWriteJournalOp2?
-    && dop.id1 !in s.reqWriteJournals
-    && dop.id1 !in s.respWriteJournals
-    && dop.id2 !in s.reqWriteJournals
-    && dop.id2 !in s.respWriteJournals
-    && ValidReqWriteJournal(dop.reqWriteJournal1)
-    && ValidReqWriteJournal(dop.reqWriteJournal2)
-    && s' == s.(reqWriteJournals :=
-        s.reqWriteJournals[dop.id1 := dop.reqWriteJournal1]
-                          [dop.id2 := dop.reqWriteJournal2]
-      )
+    && updateLoc in disk'
+    && disk'[updateLoc] == t
+    && (forall loc | loc in disk && !overlap(loc, updateLoc) :: loc in disk' && disk'[loc] == disk[loc])
+    && (forall loc | loc in disk' && !overlap(loc, updateLoc) :: loc in disk)
   }
 
   predicate RecvWriteIndirectionTable(k: Constants, s: Variables, s': Variables, dop: DiskOp)
   {
     && dop.ReqWriteIndirectionTableOp?
     && dop.id !in s.reqWriteIndirectionTables
-    && dop.id !in s.respWriteIndirectionTables
-    && s' == s.(reqWriteIndirectionTables := s.reqWriteIndirectionTables[dop.id := dop.reqWriteIndirectionTable])
+    && DiskMapUpdate(s.indirectionTables, s'.indirectionTables, dop.reqWriteIndirectionTable.loc, dop.reqWriteIndirectionTable.indirectionTable)
+    && s' == s.(reqWriteIndirectionTables := s.reqWriteIndirectionTables[dop.id := dop.reqWriteIndirectionTable.loc])
+              .(indirectionTables := s'.indirectionTables)
   }
 
   predicate RecvWriteNode(k: Constants, s: Variables, s': Variables, dop: DiskOp)
   {
     && dop.ReqWriteNodeOp?
     && dop.id !in s.reqWriteNodes
-    && dop.id !in s.respWriteNodes
-    && s' == s.(reqWriteNodes := s.reqWriteNodes[dop.id := dop.reqWriteNode])
+    && DiskMapUpdate(s.nodes, s'.nodes, dop.reqWriteNode.loc, dop.reqWriteNode.node)
+    && s' == s.(reqWriteNodes := s.reqWriteNodes[dop.id := dop.reqWriteNode.loc])
+              .(nodes := s'.nodes)
   }
 
   ///////// AckRead
@@ -240,41 +206,59 @@ module AsyncSectorDisk {
     && dop.RespReadSuperblockOp?
     && (dop.which == 0 || dop.which == 1)
     && (dop.which == 0 ==>
-      && s.respReadSuperblock1.Some?
-      && dop.id == s.respReadSuperblock1.value.id
-      && dop.superblock == s.respReadSuperblock1.value.superblock
-      && s' == s.(respReadSuperblock1 := None)
+      && s.reqReadSuperblock1.Some?
+      && dop.id == s.reqReadSuperblock1.value
+      && (dop.superblock.Some? ==> dop.superblock == s.superblock1)
+      && s' == s.(reqReadSuperblock1 := None)
     )
     && (dop.which == 1 ==>
-      && s.respReadSuperblock2.Some?
-      && dop.id == s.respReadSuperblock2.value.id
-      && dop.superblock == s.respReadSuperblock2.value.superblock
-      && s' == s.(respReadSuperblock2 := None)
+      && s.reqReadSuperblock2.Some?
+      && dop.id == s.reqReadSuperblock2.value
+      && (dop.superblock.Some? ==> dop.superblock == s.superblock2)
+      && s' == s.(reqReadSuperblock2 := None)
+    )
+  }
+
+  function {:opaque} journalRead(a: seq<Option<JournalBlock>>) : Option<seq<JournalBlock>>
+  {
+    if a == [] then Some([]) else (
+      var p := journalRead(DropLast(a));
+      if p.Some? && Last(a).Some? then
+        Some(p.value + [Last(a).value])
+      else
+        None
     )
   }
 
   predicate AckReadJournal(k: Constants, s: Variables, s': Variables, dop: DiskOp)
   {
     && dop.RespReadJournalOp?
-    && dop.id in s.respReadJournals
-    && s.respReadJournals[dop.id] == dop.journal
-    && s' == s.(respReadJournals := MapRemove1(s.respReadJournals, dop.id))
+    && dop.id in s.reqReadJournals
+    && var req := s.reqReadJournals[dop.id];
+    && 0 <= req.start <= req.start + req.len <= |s.journal|
+    && (dop.journal.Some? ==>
+      dop.journal == journalRead(s.journal[req.start .. req.start + req.len]))
+    && s' == s.(reqReadJournals := MapRemove1(s.reqReadJournals, dop.id))
   }
 
   predicate AckReadIndirectionTable(k: Constants, s: Variables, s': Variables, dop: DiskOp)
   {
     && dop.RespReadIndirectionTableOp?
-    && dop.id in s.respReadIndirectionTables
-    && s.respReadIndirectionTables[dop.id] == dop.indirectionTable
-    && s' == s.(respReadIndirectionTables := MapRemove1(s.respReadIndirectionTables, dop.id))
+    && dop.id in s.reqReadIndirectionTables
+    && var req := s.reqReadIndirectionTables[dop.id];
+    && (dop.indirectionTable.Some? ==>
+      dop.indirectionTable == ImapLookupOption(s.indirectionTables, req.loc))
+    && s' == s.(reqReadIndirectionTables := MapRemove1(s.reqReadIndirectionTables, dop.id))
   }
 
   predicate AckReadNode(k: Constants, s: Variables, s': Variables, dop: DiskOp)
   {
     && dop.RespReadNodeOp?
-    && dop.id in s.respReadNodes
-    && s.respReadNodes[dop.id] == dop.node
-    && s' == s.(respReadNodes := MapRemove1(s.respReadNodes, dop.id))
+    && dop.id in s.reqReadNodes
+    && var req := s.reqReadNodes[dop.id];
+    && (dop.node.Some? ==>
+      dop.node == ImapLookupOption(s.nodes, req.loc))
+    && s' == s.(reqReadNodes := MapRemove1(s.reqReadNodes, dop.id))
   }
 
   ///////// AckWrite
@@ -284,36 +268,36 @@ module AsyncSectorDisk {
     && dop.RespWriteSuperblockOp?
     && (dop.which == 0 || dop.which == 1)
     && (dop.which == 0 ==>
-      && s.respWriteSuperblock1.Some?
-      && dop.id == s.respWriteSuperblock1.value
-      && s' == s.(respWriteSuperblock1 := None)
+      && s.reqWriteSuperblock1.Some?
+      && dop.id == s.reqWriteSuperblock1.value
+      && s' == s.(reqWriteSuperblock1 := None)
     )
     && (dop.which == 1 ==>
-      && s.respWriteSuperblock2.Some?
-      && dop.id == s.respWriteSuperblock2.value
-      && s' == s.(respWriteSuperblock2 := None)
+      && s.reqWriteSuperblock2.Some?
+      && dop.id == s.reqWriteSuperblock2.value
+      && s' == s.(reqWriteSuperblock2 := None)
     )
   }
 
   predicate AckWriteJournal(k: Constants, s: Variables, s': Variables, dop: DiskOp)
   {
     && dop.RespWriteJournalOp?
-    && dop.id in s.respWriteJournals
-    && s' == s.(respWriteJournals := s.respWriteJournals - {dop.id})
+    && dop.id in s.reqWriteJournals
+    && s' == s.(reqWriteJournals := MapRemove1(s.reqWriteJournals, dop.id))
   }
 
   predicate AckWriteIndirectionTable(k: Constants, s: Variables, s': Variables, dop: DiskOp)
   {
     && dop.RespWriteIndirectionTableOp?
-    && dop.id in s.respWriteIndirectionTables
-    && s' == s.(respWriteIndirectionTables := s.respWriteIndirectionTables - {dop.id})
+    && dop.id in s.reqWriteIndirectionTables
+    && s' == s.(reqWriteIndirectionTables := MapRemove1(s.reqWriteIndirectionTables, dop.id))
   }
 
   predicate AckWriteNode(k: Constants, s: Variables, s': Variables, dop: DiskOp)
   {
     && dop.RespWriteNodeOp?
-    && dop.id in s.respWriteNodes
-    && s' == s.(respWriteNodes := s.respWriteNodes - {dop.id})
+    && dop.id in s.reqWriteNodes
+    && s' == s.(reqWriteNodes := MapRemove1(s.reqWriteNodes, dop.id))
   }
 
   //// Stutter
@@ -332,7 +316,6 @@ module AsyncSectorDisk {
 
     && (dop.ReqWriteSuperblockOp? ==> RecvWriteSuperblock(k, s, s', dop))
     && (dop.ReqWriteJournalOp? ==> RecvWriteJournal(k, s, s', dop))
-    && (dop.ReqWriteJournalOp2? ==> RecvWriteJournal2(k, s, s', dop))
     && (dop.ReqWriteIndirectionTableOp? ==> RecvWriteIndirectionTable(k, s, s', dop))
     && (dop.ReqWriteNodeOp? ==> RecvWriteNode(k, s, s', dop))
 
@@ -349,216 +332,68 @@ module AsyncSectorDisk {
     && (dop.NoDiskOp? ==> Stutter(k, s, s', dop))
   }
 
-  datatype InternalStep =
-    | ProcessReadSuperblockStep(which: int, id: ReqId)
-    | ProcessReadJournalStep(id: ReqId)
-    | ProcessReadIndirectionTableStep(id: ReqId)
-    | ProcessReadNodeStep(id: ReqId)
-
-    | ProcessReadFailureSuperblockStep(which: int, id: ReqId)
-    | ProcessReadFailureJournalStep(id: ReqId)
-    | ProcessReadFailureIndirectionTableStep(id: ReqId)
-    | ProcessReadFailureNodeStep(id: ReqId)
-
-    | ProcessWriteSuperblockStep(which: int, id: ReqId)
-    | ProcessWriteJournalStep(id: ReqId)
-    | ProcessWriteIndirectionTableStep(id: ReqId)
-    | ProcessWriteNodeStep(id: ReqId)
-
-  ///////// ProcessRead
-
-  predicate ProcessReadSuperblock(k: Constants, s: Variables, s': Variables, which: int, id: ReqId)
+  predicate havocSuperblockWrite(superblock: Option<Superblock>, superblock': Option<Superblock>, reqWriteSuperblock: Option<ReqId>)
   {
-    && (which == 0 || which == 1)
-    && (which == 0 ==>
-      && s.reqReadSuperblock1 == Some(id)
-      && s' == s.(reqReadSuperblock1 := None)
-                .(respReadSuperblock1 := Some(RespReadSuperblockId(id, s.superblock1)))
-    )
-    && (which == 1 ==>
-      && s.reqReadSuperblock2 == Some(id)
-      && s' == s.(reqReadSuperblock2 := None)
-                .(respReadSuperblock2 := Some(RespReadSuperblockId(id, s.superblock2)))
-    )
+    reqWriteSuperblock.None? ==> superblock == superblock'
   }
 
-  function {:opaque} journalRead(a: seq<Option<JournalBlock>>) : Option<seq<JournalBlock>>
+  predicate JournalUntouched(
+    i: int, 
+    reqWriteJournals: map<ReqId, JournalIndices>)
   {
-    if a == [] then Some([]) else (
-      var p := journalRead(DropLast(a));
-      if p.Some? && Last(a).Some? then
-        Some(p.value + [Last(a).value])
-      else
-        None
-    )
+    forall id | id in reqWriteJournals ::
+        !InCyclicRange(i, reqWriteJournals[id])
   }
 
-  predicate ProcessReadJournal(k: Constants, s: Variables, s': Variables, id: ReqId)
+  predicate havocJournal(
+    journal: seq<Option<JournalBlock>>,
+    journal': seq<Option<JournalBlock>>,
+    reqWriteJournals: map<ReqId, JournalIndices>)
   {
-    && id in s.reqReadJournals
-    && var req := s.reqReadJournals[id];
-    && 0 <= req.start <= req.start + req.len <= |s.journal|
-    && var jr := journalRead(s.journal[req.start .. req.start + req.len]);
-    && s' == s.(reqReadJournals := MapRemove1(s.reqReadJournals, id))
-              .(respReadJournals := s.respReadJournals[id := jr])
+    && |journal'| == |journal|
+    && forall i | 0 <= i < |journal| ::
+        JournalUntouched(i, reqWriteJournals) ==>
+            journal[i] == journal'[i]
   }
 
-  predicate ProcessReadIndirectionTable(k: Constants, s: Variables, s': Variables, id: ReqId)
+  predicate UntouchedLoc(loc: Location, reqs: map<ReqId, Location>)
   {
-    && id in s.reqReadIndirectionTables
-    && var req := s.reqReadIndirectionTables[id];
-    && s' == s.(reqReadIndirectionTables := MapRemove1(s.reqReadIndirectionTables, id))
-              .(respReadIndirectionTables := s.respReadIndirectionTables[id := ImapLookupOption(s.indirectionTables, req.loc)])
+    forall id | id in reqs :: !overlap(loc, reqs[id])
   }
 
-  predicate ProcessReadNode(k: Constants, s: Variables, s': Variables, id: ReqId)
+  predicate havocMap<T>(
+    m: imap<Location, T>,
+    m': imap<Location, T>,
+    reqs: map<ReqId, Location>)
   {
-    && id in s.reqReadNodes
-    && var req := s.reqReadNodes[id];
-    && s' == s.(reqReadNodes := MapRemove1(s.reqReadNodes, id))
-              .(respReadNodes := s.respReadNodes[id := ImapLookupOption(s.nodes, req.loc)])
-  }
-
-  ////////// ProcessReadFailure
-
-  predicate ProcessReadFailureSuperblock(k: Constants, s: Variables, s': Variables, which: int, id: ReqId)
-  {
-    && (which == 0 || which == 1)
-    && (which == 0 ==>
-      && s.reqReadSuperblock1 == Some(id)
-      && s' == s.(reqReadSuperblock1 := None)
-                .(respReadSuperblock1 := Some(RespReadSuperblockId(id, None)))
-    )
-    && (which == 1 ==>
-      && s.reqReadSuperblock2 == Some(id)
-      && s' == s.(reqReadSuperblock2 := None)
-                .(respReadSuperblock2 := Some(RespReadSuperblockId(id, None)))
-    )
-  }
-
-  predicate ProcessReadFailureJournal(k: Constants, s: Variables, s': Variables, id: ReqId)
-  {
-    && id in s.reqReadJournals
-    && s' == s.(reqReadJournals := MapRemove1(s.reqReadJournals, id))
-              .(respReadJournals := s.respReadJournals[id := None])
-  }
-
-  predicate ProcessReadFailureIndirectionTable(k: Constants, s: Variables, s': Variables, id: ReqId)
-  {
-    && id in s.reqReadIndirectionTables
-    && s' == s.(reqReadIndirectionTables := MapRemove1(s.reqReadIndirectionTables, id))
-              .(respReadIndirectionTables := s.respReadIndirectionTables[id := None])
-  }
-
-  predicate ProcessReadFailureNode(k: Constants, s: Variables, s': Variables, id: ReqId)
-  {
-    && id in s.reqReadNodes
-    && s' == s.(reqReadNodes := MapRemove1(s.reqReadNodes, id))
-              .(respReadNodes := s.respReadNodes[id := None])
-  }
-
-  //////// ProcessWrite
-
-  predicate ProcessWriteSuperblock(k: Constants, s: Variables, s': Variables, which: int, id: ReqId)
-  {
-    && (which == 0 || which == 1)
-    && (which == 0 ==>
-      && s.reqWriteSuperblock1.Some?
-      && s.reqWriteSuperblock1.value.id == id
-      && s' == s.(superblock1 := Some(s.reqWriteSuperblock1.value.req.superblock))
-                .(reqWriteSuperblock1 := None)
-                .(respWriteSuperblock1 := Some(id))
-    )
-    && (which == 1 ==>
-      && s.reqWriteSuperblock2.Some?
-      && s.reqWriteSuperblock2.value.id == id
-      && s' == s.(superblock2 := Some(s.reqWriteSuperblock2.value.req.superblock))
-                .(reqWriteSuperblock2 := None)
-                .(respWriteSuperblock2 := Some(id))
-    )
-  }
-
-  predicate ProcessWriteJournal(k: Constants, s: Variables, s': Variables, which: int, id: ReqId)
-  {
-    && (which == 0 || which == 1)
-    && (which == 0 ==>
-      && s.reqWriteSuperblock1.Some?
-      && s.reqWriteSuperblock1.value.id == id
-      && s' == s.(superblock1 := Some(s.reqWriteSuperblock1.value.req.superblock))
-                .(reqWriteSuperblock1 := None)
-                .(respWriteSuperblock1 := Some(id))
-    )
-    && (which == 1 ==>
-      && s.reqWriteSuperblock2.Some?
-      && s.reqWriteSuperblock2.value.id == id
-      && s' == s.(superblock2 := Some(s.reqWriteSuperblock2.value.req.superblock))
-                .(reqWriteSuperblock2 := None)
-                .(respWriteSuperblock2 := Some(id))
-    )
-  }
-
-  predicate ProcessWriteIndirectionTable(k: Constants, s: Variables, s': Variables, id: ReqId)
-  {
-    && id in s.reqWriteIndirectionTables
-    && var req := s.reqWriteIndirectionTables[id];
-    && s' == s.(reqWriteIndirectionTables := MapRemove1(s.reqWriteIndirectionTables, id))
-              .(respWriteIndirectionTables := s.respWriteIndirectionTables + {id})
-              .(indirectionTables := s'.indirectionTables)
-
-    && req.loc in s'.indirectionTables
-    && s'.indirectionTables[req.loc] == req.indirectionTable
-    && (forall loc | loc in s.indirectionTables && !overlap(loc, req.loc) :: loc in s'.indirectionTables && s'.indirectionTables[loc] == s.indirectionTables[loc])
-    && (forall loc | loc in s'.indirectionTables && !overlap(loc, req.loc) :: loc in s.indirectionTables)
-  }
-
-  predicate ProcessWriteNode(k: Constants, s: Variables, s': Variables, id: ReqId)
-  {
-    && id in s.reqWriteNodes
-    && var req := s.reqWriteNodes[id];
-    && s' == s.(reqWriteNodes := MapRemove1(s.reqWriteNodes, id))
-              .(respWriteNodes := s.respWriteNodes + {id})
-              .(nodes := s'.nodes)
-
-    // It would be easier to say s'.nodes == s.nodes[req.loc := req.sector]
-    // but to make the refinement from AsyncDiskModel easier, we only require that
-    // the map preserves every location not intersecting the given region. We don't
-    // have to say anything about potential intervals which could intersect this one.
-    && req.loc in s'.nodes
-    && s'.nodes[req.loc] == req.node
-    && (forall loc | loc in s.nodes && !overlap(loc, req.loc) :: loc in s'.nodes && s'.nodes[loc] == s.nodes[loc])
-    && (forall loc | loc in s'.nodes && !overlap(loc, req.loc) :: loc in s.nodes)
-  }
-
-  predicate NextInternalStep(k: Constants, s: Variables, s': Variables, step: InternalStep)
-  {
-    match step {
-      case ProcessReadSuperblockStep(which, id) => ProcessReadSuperblock(k, s, s', which, id)
-      case ProcessReadJournalStep(id) => ProcessReadJournal(k, s, s', id)
-      case ProcessReadIndirectionTableStep(id) => ProcessReadIndirectionTable(k, s, s', id)
-      case ProcessReadNodeStep(id) => ProcessReadNode(k, s, s', id)
-      case ProcessReadFailureSuperblockStep(which, id) => ProcessReadFailureSuperblock(k, s, s', which, id)
-      case ProcessReadFailureJournalStep(id) => ProcessReadFailureJournal(k, s, s', id)
-      case ProcessReadFailureIndirectionTableStep(id) => ProcessReadFailureIndirectionTable(k, s, s', id)
-      case ProcessReadFailureNodeStep(id) => ProcessReadFailureNode(k, s, s', id)
-      case ProcessWriteSuperblockStep(which, id) => ProcessWriteSuperblock(k, s, s', which, id)
-      case ProcessWriteJournalStep(id) => ProcessWriteJournal(k, s, s', id)
-      case ProcessWriteIndirectionTableStep(id) => ProcessWriteIndirectionTable(k, s, s', id)
-      case ProcessWriteNodeStep(id) => ProcessWriteNode(k, s, s', id)
-    }
-  }
-
-  predicate NextInternal(k: Constants, s: Variables, s': Variables)
-  {
-    exists step :: NextInternalStep(k, s, s', step)
+    forall loc | loc in m ::
+        UntouchedLoc(loc, reqs) ==>
+            loc in m' && m'[loc] == m[loc]
   }
 
   predicate Crash(k: Constants, s: Variables, s': Variables)
   {
-    s' == Variables(map[], map[], map[], map[], s.blocks)
+    && s.reqReadSuperblock1 == None
+    && s.reqReadSuperblock2 == None
+    && s.reqReadJournals == map[]
+    && s.reqReadIndirectionTables == map[]
+    && s.reqReadNodes == map[]
+
+    && s.reqWriteSuperblock1 == None
+    && s.reqWriteSuperblock2 == None
+    && s.reqWriteJournals == map[]
+    && s.reqWriteIndirectionTables == map[]
+    && s.reqWriteNodes == map[]
+
+    && havocSuperblockWrite(s.superblock1, s'.superblock1, s.reqWriteSuperblock1)
+    && havocSuperblockWrite(s.superblock2, s'.superblock2, s.reqWriteSuperblock2)
+    && havocJournal(s.journal, s'.journal, s.reqWriteJournals)
+    && havocMap(s.indirectionTables, s'.indirectionTables, s.reqWriteIndirectionTables)
+    && havocMap(s.nodes, s'.nodes, s.reqWriteNodes)
   }
 }
 
-/*abstract module AsyncSectorDiskMachine {
+abstract module AsyncSectorDiskMachine {
   import D = AsyncSectorDisk
   import UI
 
@@ -568,14 +403,8 @@ module AsyncSectorDisk {
   type Sector
   type UIOp = UI.Op
 
-  type DiskOp = D.DiskOp
-  type ReqRead = D.ReqRead
-  type ReqWrite = D.ReqWrite
-  type RespRead = D.RespRead
-  type RespWrite = D.RespWrite
-
   predicate Init(k: Constants, s: Variables)
-  predicate Next(k: Constants, s: Variables, s': Variables, uiop: UIOp, dop: DiskOp)
+  predicate Next(k: Constants, s: Variables, s': Variables, uiop: UIOp, dop: D.DiskOp)
 }
 
 // A disk attached to a program ("Machine"), modeling the nondeterministic crashes that reset the
@@ -587,27 +416,18 @@ abstract module AsyncSectorDiskModel {
   import AsyncSectorDiskModelTypes
   import opened SectorType
 
-  type DiskOp = M.DiskOp
   type Constants = AsyncSectorDiskModelTypes.AsyncSectorDiskModelConstants<M.Constants, D.Constants>
   type Variables = AsyncSectorDiskModelTypes.AsyncSectorDiskModelVariables<M.Variables, D.Variables>
   type UIOp = M.UIOp
 
   datatype Step =
-    | MachineStep(dop: DiskOp)
-    | DiskInternalStep(step: D.InternalStep)
+    | MachineStep(dop: D.DiskOp)
     | CrashStep
   
-  predicate Machine(k: Constants, s: Variables, s': Variables, uiop: UIOp, dop: DiskOp)
+  predicate Machine(k: Constants, s: Variables, s': Variables, uiop: UIOp, dop: D.DiskOp)
   {
     && M.Next(k.machine, s.machine, s'.machine, uiop, dop)
     && D.Next(k.disk, s.disk, s'.disk, dop)
-  }
-
-  predicate DiskInternal(k: Constants, s: Variables, s': Variables, uiop: UIOp, step: D.InternalStep)
-  {
-    && uiop.NoOp?
-    && s.machine == s'.machine
-    && D.NextInternalStep(k.disk, s.disk, s'.disk, step)
   }
 
   predicate Crash(k: Constants, s: Variables, s': Variables, uiop: UIOp)
@@ -621,7 +441,6 @@ abstract module AsyncSectorDiskModel {
   {
     match step {
       case MachineStep(dop) => Machine(k, s, s', uiop, dop)
-      case DiskInternalStep(step) => DiskInternal(k, s, s', uiop, step)
       case CrashStep => Crash(k, s, s', uiop)
     }
   }
@@ -641,4 +460,4 @@ abstract module AsyncSectorDiskModel {
     requires Inv(k, s)
     requires Next(k, s, s', uiop)
     ensures Inv(k, s')
-}*/
+}
