BlockCacheSystem/JournalDisk.i.dfy
@@ -1,0 +1,60 @@
+include "JournalRange.i.dfy"
+include "DiskLayout.i.dfy"
+
+module JournalDisk {
+  import opened DiskLayout
+  import opened JournalRanges
+  import opened Options
+
+  datatype JournalIndices = JournalIndices(start: int, len: int)
+
+  predicate ValidJournalIndices(indices: JournalIndices)
+  {
+    && 0 <= indices.start < NumJournalBlocks() as int
+    && 0 <= indices.len <= NumJournalBlocks() as int
+  }
+
+  predicate ValidJournal(journal: seq<Option<JournalBlock>>)
+  {
+    |journal| == NumJournalBlocks() as int
+  }
+
+  function CyclicSliceValue(
+    journal: seq<Option<JournalBlock>>,
+    indices: JournalIndices,
+    newEntries: seq<JournalBlock>,
+    i: int
+  ) : Option<JournalBlock>
+  requires ValidJournal(journal)
+  requires ValidJournalIndices(indices)
+  requires indices.len == |newEntries|
+  requires 0 <= i < NumJournalBlocks() as int
+  {
+    if indices.start <= i < indices.start + indices.len then
+      Some(newEntries[i - indices.start])
+    else if indices.start <= i + NumJournalBlocks() as int < indices.start + indices.len then
+      Some(newEntries[i + NumJournalBlocks() as int - indices.start])
+    else
+      journal[i]
+  }
+
+  predicate {:opaque} JournalUpdate(
+      journal: seq<Option<JournalBlock>>,
+      journal': seq<Option<JournalBlock>>,
+      indices: JournalIndices,
+      newEntries: seq<JournalBlock>)
+  {
+    && ValidJournal(journal)
+    && ValidJournal(journal')
+    && ValidJournalIndices(indices)
+    && indices.len == |newEntries|
+    && (forall i | 0 <= i < |journal| ::
+        journal'[i] == CyclicSliceValue(journal, indices, newEntries, i))
+  }
+
+  predicate InCyclicRange(i: int, indices: JournalIndices)
+  {
+    || (indices.start <= i < indices.start + indices.len)
+    || (indices.start <= i + NumJournalBlocks() as int < indices.start + indices.len)
+  }
+}
